secure_api/merkle_tree/MerkleTree.New.Low.Serialization.fst
@@ -1,0 +1,322 @@
+module MerkleTree.New.Low.Serialization
+
+open FStar.Integers
+open FStar.Mul
+open LowStar.Modifies
+open LowStar.BufferOps
+open LowStar.Vector
+open LowStar.RVector
+open LowStar.Regional
+open LowStar.Regional.Instances
+
+open MerkleTree.New.Low
+
+module HS = FStar.HyperStack
+module HST = FStar.HyperStack.ST
+
+module B = LowStar.Buffer
+module V = LowStar.Vector
+module RV = LowStar.RVector
+module RVI = LowStar.Regional.Instances
+
+module U16 = FStar.UInt16
+module U32 = FStar.UInt32
+module U64 = FStar.UInt64
+module U8 = FStar.UInt8
+
+let uint8_t = U8.t
+let uint16_t = U16.t
+let uint32_t = U32.t
+let uint64_t = U64.t
+
+let uint8_p = B.buffer uint8_t
+
+
+#reset-options "--z3rlimit 5 --initial_fuel 1 --max_fuel 1 --initial_ifuel 0 --max_ifuel 0"
+
+private let serialize_bool (x:bool) (buf:uint8_p) (sz:uint32_t{B.len buf = sz}) (pos:uint32_t) : HST.ST (bool & uint32_t)
+  (requires (fun h0 -> B.live h0 buf))
+  (ensures (fun h0 _ h1 -> B.live h1 buf /\ modifies (B.loc_buffer buf) h0 h1))
+= if pos >= sz then (false, 0ul)
+  else begin
+    B.upd buf pos (if x then 1uy else 0uy);
+    (true, pos + 1ul)
+  end
+
+private let serialize_uint8_t (x:uint8_t) (buf:uint8_p) (sz:uint32_t{B.len buf = sz}) (pos:uint32_t) : HST.ST (bool & uint32_t)
+  (requires (fun h0 -> B.live h0 buf))
+  (ensures (fun h0 _ h1 -> B.live h1 buf /\ modifies (B.loc_buffer buf) h0 h1))
+= if pos >= sz then (false, 0ul)
+  else begin B.upd buf pos x;
+    (true, pos + 1ul)
+  end
+
+private let serialize_uint16_t (x:uint16_t) (buf:uint8_p) (sz:uint32_t{B.len buf = sz}) (pos:uint32_t) : HST.ST (bool & uint32_t)
+  (requires (fun h0 -> B.live h0 buf))
+  (ensures (fun h0 _ h1 -> B.live h1 buf /\ modifies (B.loc_buffer buf) h0 h1))
+= let _, pos = serialize_uint8_t (Int.Cast.uint16_to_uint8 (U16.shift_right x 8ul)) buf sz pos in
+  serialize_uint8_t (Int.Cast.uint16_to_uint8 x) buf sz pos
+
+private let serialize_uint32_t (x:uint32_t) (buf:uint8_p) (sz:uint32_t{B.len buf = sz}) (pos:uint32_t) : HST.ST (bool & uint32_t)
+  (requires (fun h0 -> B.live h0 buf))
+  (ensures (fun h0 _ h1 -> B.live h1 buf /\ modifies (B.loc_buffer buf) h0 h1))
+= let _, pos = serialize_uint16_t (Int.Cast.uint32_to_uint16 (U32.shift_right x 16ul)) buf sz pos in
+  serialize_uint16_t (Int.Cast.uint32_to_uint16 x) buf sz pos
+
+private let serialize_uint64_t (x:uint64_t) (buf:uint8_p) (sz:uint32_t{B.len buf = sz}) (pos:uint32_t) : HST.ST (bool & uint32_t)
+  (requires (fun h0 -> B.live h0 buf))
+  (ensures (fun h0 _ h1 -> B.live h1 buf /\ modifies (B.loc_buffer buf) h0 h1))
+= let _, pos = serialize_uint32_t (Int.Cast.uint64_to_uint32 (U64.shift_right x 32ul)) buf sz pos in
+  serialize_uint32_t (Int.Cast.uint64_to_uint32 x) buf sz pos
+
+private let serialize_offset_t = serialize_uint64_t
+private let serialize_index_t = serialize_uint32_t
+
+private let serialize_hash (x:hash) (buf:uint8_p) (sz:uint32_t{B.len buf = sz}) (pos:uint32_t) : HST.ST (bool & uint32_t)
+  (requires (fun h0 -> B.live h0 buf /\ B.live h0 x /\ B.len x = hash_size))
+  (ensures (fun h0 _ h1 -> B.live h1 buf /\ B.live h1 x /\ modifies (B.loc_buffer buf) h0 h1))
+= if pos >= sz then (false, 0ul)
+  else begin
+    let rec serialize_hash_i pos (i:uint32_t): HST.ST (bool & uint32_t)
+        (requires (fun h0 -> B.live h0 buf /\ B.live h0 x /\ B.len x = hash_size))
+        (ensures (fun h0 _ h1 -> B.live h1 buf /\ B.live h1 x /\ modifies (B.loc_buffer buf) h0 h1))
+    = if pos >= sz then (false, 0ul)
+      else if i >= hash_size then (true, pos)
+      else begin
+        let _, pos = serialize_uint8_t (B.index x i) buf sz pos in
+        serialize_hash_i pos (i+1ul)
+      end in
+    serialize_hash_i pos 0ul
+  end
+
+private unfold let hash_vec_bytes (v:hash_vec) = 4UL + U64.mul (u32_64 (V.size_of v)) (u32_64 hash_size)
+
+private let serialize_hash_vec (x:hash_vec) (buf:uint8_p) (sz:uint32_t{B.len buf = sz}) (pos:uint32_t) : HST.ST (bool & uint32_t)
+  (requires (fun h0 -> B.live h0 buf /\ V.live h0 x))
+  (ensures (fun h0 _ h1 -> B.live h1 buf /\ V.live h1 x /\ modifies (B.loc_buffer buf) h0 h1))
+= if pos >= sz then (false, 0ul)
+  else begin
+    let rec serialize_hash_vec_i pos (i:uint32_t): HST.ST (bool & uint32_t)
+      (requires (fun h0 -> B.live h0 buf /\ V.live h0 x))
+      (ensures (fun h0 _ h1 -> B.live h1 buf /\ V.live h1 x /\ modifies (B.loc_buffer buf) h0 h1))
+    = if pos >= sz then (false, 0ul)
+      else if i >= V.size_of x then (true, pos)
+      else begin
+        let vi = V.index x i in
+        let h0 = HST.get() in
+        assume (B.live h0 vi /\ B.len vi = hash_size);
+        let _, pos = serialize_hash vi buf sz pos in
+        serialize_hash_vec_i pos (i+1ul)
+      end in
+    let _, pos = serialize_uint32_t (V.size_of x) buf sz pos in
+    serialize_hash_vec_i pos 0ul
+  end
+
+private let rec hash_vv_bytes (vv:hash_vv{V.size_of vv = merkle_tree_size_lg}): HST.ST uint64_t
+  (requires (fun h0 -> V.live h0 vv))
+  (ensures (fun h0 _ h1 -> h0 == h1 /\ V.live h1 vv))
+= let rec hash_vv_bytes_i (vv:hash_vv) (i:uint32_t): HST.ST uint64_t
+    (requires (fun h0 -> V.live h0 vv))
+    (ensures (fun h0 _ h1 -> h0 == h1 /\ V.live h1 vv))
+  = if i >= V.size_of vv then 4UL
+    else begin
+      let vvi = V.index vv i in
+      let r = hash_vec_bytes vvi in
+      let rest = hash_vv_bytes_i vv (i+1ul) in
+      if uint64_max - rest < r then uint64_max
+      else rest + r
+    end in
+  hash_vv_bytes_i vv 0ul
+
+private let serialize_hash_vv (x:hash_vv) (buf:uint8_p) (sz:uint32_t{B.len buf = sz}) (pos:uint32_t): HST.ST (bool & uint32_t)
+  (requires (fun h0 -> B.live h0 buf /\ V.live h0 x))
+  (ensures (fun h0 _ h1 -> B.live h1 buf /\ V.live h1 x /\ modifies (B.loc_buffer buf) h0 h1))
+= if pos >= sz then (false, 0ul)
+  else begin
+    let rec serialize_hash_vv_i pos (i:uint32_t): HST.ST (bool & uint32_t)
+      (requires (fun h0 -> B.live h0 buf /\ V.live h0 x))
+      (ensures (fun h0 _ h1 -> B.live h1 buf /\ V.live h1 x /\ modifies (B.loc_buffer buf) h0 h1))
+    = if pos >= sz then (false, 0ul)
+      else if i >= V.size_of x then (true, pos)
+      else begin
+        let vi = V.index x i in
+        let h0 = HST.get() in
+        assume (V.live h0 vi);
+        let _, pos = serialize_hash_vec vi buf sz pos in
+        serialize_hash_vv_i pos (i+1ul)
+      end in
+    let _, pos = serialize_uint32_t (V.size_of x) buf sz pos in
+    serialize_hash_vv_i pos 0ul
+  end
+
+
+private let deserialize_bool (buf:uint8_p) (sz:uint32_t{B.len buf = sz}) (pos:uint32_t): HST.ST (bool & uint32_t & bool)
+  (requires (fun h0 -> B.live h0 buf))
+  (ensures (fun _ _ h1 -> B.live h1 buf))
+= if pos >= sz then (false, pos, false)
+  else (true, pos + 1ul, (match B.index buf pos with| 0uy -> false | _ -> true))
+
+private let deserialize_uint8_t (buf:uint8_p) (sz:uint32_t{B.len buf = sz}) (pos:uint32_t): HST.ST (bool & uint32_t & uint8_t)
+  (requires (fun h0 -> B.live h0 buf))
+  (ensures (fun _ _ h1 -> B.live h1 buf))
+= if pos >= sz then (false, pos, 0uy)
+  else (true, pos + 1ul, B.index buf pos)
+
+private let deserialize_uint16_t (buf:uint8_p) (sz:uint32_t{B.len buf = sz}) (pos:uint32_t): HST.ST (bool & uint32_t & uint16_t)
+  (requires (fun h0 -> B.live h0 buf))
+  (ensures (fun _ _ h1 -> B.live h1 buf))
+= if pos >= sz then (false, pos, 0us)
+  else begin
+    let _, pos, b0 = deserialize_uint8_t buf sz pos in
+    let k, pos, b1 = deserialize_uint8_t buf sz pos in
+    (k, pos, (U16.shift_left (Int.Cast.uint8_to_uint16 b0) 8ul) + Int.Cast.uint8_to_uint16 b1)
+  end
+
+private let deserialize_uint32_t (buf:uint8_p) (sz:uint32_t{B.len buf = sz}) (pos:uint32_t): HST.ST (bool & uint32_t & uint32_t)
+  (requires (fun h0 -> B.live h0 buf))
+  (ensures (fun _ _ h1 -> B.live h1 buf))
+= if pos >= sz then (false, pos, 0ul)
+  else begin
+    let _, pos, b0 = deserialize_uint16_t buf sz pos in
+    let k, pos, b1 = deserialize_uint16_t buf sz pos in
+    (k, pos, (U32.shift_left (Int.Cast.uint16_to_uint32 b0) 16ul) + Int.Cast.uint16_to_uint32 b1)
+  end
+
+private let deserialize_uint64_t (buf:uint8_p) (sz:uint32_t{B.len buf = sz}) (pos:uint32_t): HST.ST (bool & uint32_t & uint64_t)
+  (requires (fun h0 -> B.live h0 buf))
+  (ensures (fun _ _ h1 -> B.live h1 buf))
+= if pos >= sz then (false, pos, 0UL)
+  else begin
+    let _, pos, b0 = deserialize_uint32_t buf sz pos in
+    let k, pos, b1 = deserialize_uint32_t buf sz pos in
+    (k, pos, (U64.shift_left (u32_64 b0) 32ul) + u32_64 b1)
+  end
+
+private let deserialize_offset_t = deserialize_uint64_t
+private let deserialize_index_t = deserialize_uint32_t
+
+private let deserialize_hash (buf:uint8_p) (sz:uint32_t{B.len buf = sz}) (r:HST.erid) (pos:uint32_t): HST.ST (bool & uint32_t & hash)
+  (requires (fun h0 -> B.live h0 buf))
+  (ensures (fun h0 _ h1 -> B.live h1 buf))
+= if pos >= sz then (false, pos, Rgl?.dummy hreg)
+  else begin
+    let h0 = HST.get() in
+    let hash = Rgl?.r_alloc hreg r in
+    assume (B.disjoint buf hash);
+    assume (sz - pos >= hash_size);
+    B.blit buf pos hash 0ul hash_size;
+    (true, pos, hash)
+  end
+
+private let deserialize_hash_vec (buf:uint8_p) (sz:uint32_t{B.len buf = sz}) (r:HST.erid) (pos:uint32_t): HST.ST (bool & uint32_t & hash_vec)
+  (requires (fun h0 -> B.live h0 buf))
+  (ensures (fun h0 _ h1 -> B.live h1 buf))
+= if pos >= sz then (false, pos, Rgl?.dummy hvreg)
+  else begin
+    let _, pos, n = deserialize_uint32_t buf sz pos in
+    if n = 0ul then (false, pos, V.alloc_empty hash)
+    else begin
+      let res = V.alloc n (Rgl?.dummy hreg) in
+      let rec deserialize_hash_vec_i pos (i:uint32_t): HST.ST (bool & uint32_t)
+        (requires (fun h0 -> B.live h0 buf))
+        (ensures (fun h0 _ h1 -> B.live h1 buf))
+      = if i >= V.size_of res then (true, pos)
+        else begin
+          let _, pos, h = deserialize_hash buf sz r pos in
+          let h0 = HST.get() in
+          assume (V.live h0 res);
+          V.assign res i h;
+          let h1 = HST.get() in
+          assume (B.live h1 buf);
+          deserialize_hash_vec_i pos (i+1ul)
+        end
+      in
+      let k, pos = deserialize_hash_vec_i pos 0ul in
+      (k, pos, res)
+    end
+  end
+
+private let deserialize_hash_vv (buf:uint8_p) (sz:uint32_t{B.len buf = sz}) (r:HST.erid) (pos:uint32_t): HST.ST (bool & uint32_t & hash_vv)
+  (requires (fun h0 -> B.live h0 buf))
+  (ensures (fun h0 _ h1 -> B.live h1 buf))
+= if pos >= sz then (false, pos, Rgl?.dummy hvvreg)
+  else begin
+    let _, pos, n = deserialize_uint32_t buf sz pos in
+    if n = 0ul then (false, pos, V.alloc_empty hash_vec)
+    else begin
+      let res = V.alloc n (Rgl?.dummy hvreg) in
+      let rec deserialize_hash_vv_i pos (i:uint32_t): HST.ST (bool & uint32_t)
+        (requires (fun h0 -> B.live h0 buf))
+        (ensures (fun h0 _ h1 -> B.live h1 buf))
+      = if i >= V.size_of res then (true, pos)
+        else begin
+          let _, pos, hv = deserialize_hash_vec buf sz r pos in
+          let h0 = HST.get() in
+          assume (V.live h0 res);
+          V.assign res i hv;
+          let h1 = HST.get() in
+          assume (B.live h1 buf);
+          deserialize_hash_vv_i pos (i+1ul)
+      end in
+    let k, pos = deserialize_hash_vv_i pos 0ul in
+    (k, pos, res)
+    end
+  end
+
+val mt_serialize_size: mt:mt_p -> HST.ST uint64_t
+  (requires (fun h0 -> mt_safe h0 mt))
+  (ensures (fun _ _ h1 -> True))
+let mt_serialize_size mt =
+  let mtv = !*mt in
+  let hs = MT?.hs mtv in
+  let rhs_ok = MT?.rhs_ok mtv in
+  let rhs = MT?.rhs mtv in
+  let hs_sz = hash_vv_bytes hs in
+  if hs_sz < uint32_max then
+    1UL +                // format version
+    4UL +                // hash_size
+    8UL +                // offset
+    4UL + 4UL +          // i, j
+    hs_sz +              // hs
+    1UL +                // rhs_ok
+    hash_vec_bytes rhs + // rhs
+    u32_64 hash_size     // mroot
+  else
+    uint64_max
+
+#set-options "--z3rlimit 10"
+val mt_serialize: mt:mt_p -> output:uint8_p -> sz:uint32_t -> HST.ST uint32_t
+  (requires (fun h0 -> mt_safe h0 mt /\ B.live h0 output /\ B.len output = sz))
+  (ensures (fun h0 _ h1 -> (* mt_safe h1 mt /\ *) B.live h1 output))
+let mt_serialize mt output sz =
+  let mtv = !*mt in
+  let _, pos = serialize_uint8_t 0uy output sz 0ul in // format version = 0uy
+  let _, pos = serialize_uint32_t hash_size output sz pos in
+  let _, pos = serialize_offset_t (MT?.offset mtv) output sz pos in
+  let _, pos = serialize_uint32_t (MT?.i mtv) output sz pos in
+  let _, pos = serialize_uint32_t (MT?.j mtv) output sz pos in
+  let _, pos = serialize_hash_vv (MT?.hs mtv) output sz pos in
+  let _, pos = serialize_bool (MT?.rhs_ok mtv) output sz pos in
+  let _, pos = serialize_hash_vec (MT?.rhs mtv) output sz pos in
+  let k, pos = serialize_hash (MT?.mroot mtv) output sz pos in
+  if k then pos else 0ul
+
+val mt_deserialize: rid:HST.erid -> input:uint8_p -> sz:uint32_t{B.len input = sz} -> mt:mt_p -> HST.ST bool
+  (requires (fun h0 -> B.live h0 input /\ mt_safe h0 mt))
+  (ensures (fun _ _ h1 -> B.live h1 input))
+let mt_deserialize rid input sz mt =
+  let _, pos, format_version = deserialize_uint8_t input sz 0ul in
+  let _, pos, hash_size = deserialize_uint32_t input sz pos in
+  let _, pos, offset = deserialize_offset_t input sz pos in
+  let _, pos, i = deserialize_index_t input sz pos in
+  let _, pos, j = deserialize_index_t input sz pos in
+  let _, ops, hs = deserialize_hash_vv input sz rid pos in
+  let _, pos, rhs_ok = deserialize_bool input sz pos in
+  let _, pos, rhs = deserialize_hash_vec input sz rid pos in
+  let k, pos, mroot = deserialize_hash input sz rid pos in
+  if not (merkle_tree_conditions offset i j hs rhs_ok rhs mroot)
+  then false
+  else begin
+    // mt *= MT offset i j hs rhs_ok rhs mroot;
+    k
+  end
